Re-work init condition so transitivity works
Turns out its important to assume and prove properties about loops
within a layer, since the idempotency condition is too strong to be
transitive. That is, idempotency isn't transitive but the property we
care about regarding loops is transitive, so you need to use idempotency
as a loop invariant within one layer and then strengthen it to prove
transitivity.

src/Spec/Layer.v
@@ -83,24 +83,21 @@ Section Layers.
             (c_sem.(crash_step);; c_exec_recover impl.(recover))
             (a_sem.(crash_step)).
 
-  Definition init_establishes_absr (impl: LayerImpl C_Op Op) (absr: relation AState CState unit) :=
-    test c_initP;; c_exec impl.(init) --->
+  Definition initialize (impl: LayerImpl C_Op Op) := c_exec impl.(init) + (c_sem.(rexec) impl.(init) impl.(init)).
+
+  Definition initialize_establishes_absr (impl: LayerImpl C_Op Op) (absr: relation AState CState unit) :=
+    test c_initP;; initialize impl --->
       (any (T:=unit);; test a_initP;; absr;; pure Initialized)
       (* failing initialization can do anything since a lower layer
                 might have initialized before this failure *)
-    + (any (T:=unit);; pure InitFailed) /\
-    (* idempotency for initialization *)
-    test c_initP;; c_sem.(exec_crash) impl.(init);; c_sem.(crash_step) --->
-       c_sem.(exec_crash) impl.(init);; c_sem.(crash_step);; test c_initP
-  .
+    + (any (T:=unit);; pure InitFailed).
 
   Record LayerRefinement :=
     { impl: LayerImpl C_Op Op;
       absr: relation AState CState unit;
       compile_op_ok : compile_op_refines_step impl absr;
       recovery_noop_ok : recovery_refines_crash_step impl absr;
-      (* TODO: prove implementations are well-formed *)
-      init_ok : init_establishes_absr impl absr }.
+      init_ok : initialize_establishes_absr impl absr }.
 
   Context (rf: LayerRefinement).
   Notation compile_op := rf.(impl).(compile_op).
@@ -250,15 +247,21 @@ Section Layers.
     then v <- r; pure (Some v)
     else pure None.
 
-  Definition initialize := c_exec rf.(impl).(init) + (c_sem.(rexec) rf.(impl).(init) rf.(impl).(init)).
+  Definition init_idempotent_absr (impl: LayerImpl C_Op Op) (absr: relation AState CState unit) :=
+    test c_initP;; c_exec impl.(init) --->
+                                      (any (T:=unit);; test a_initP;; absr;; pure Initialized)
+    (* failing initialization can do anything since a lower layer
+                might have initialized before this failure *)
+    + (any (T:=unit);; pure InitFailed) /\
+    (* idempotency for initialization *)
+    test c_initP;; c_sem.(exec_crash) impl.(init);; c_sem.(crash_step) --->
+                                                                       c_sem.(exec_crash) impl.(init);; c_sem.(crash_step);; test c_initP.
 
-  Theorem initialize_ok :
-    test c_initP;; initialize --->
-      (any (T:=unit);; test a_initP;; rf.(absr);; pure Initialized)
-    + (any (T:=unit);; pure InitFailed).
+  Theorem initialize_idempotent_ok impl absr :
+    init_idempotent_absr impl absr ->
+    initialize_establishes_absr impl absr.
   Proof.
-    pose unfolded rf.(init_ok)
-                       (fun H => red in H).
+    unfold init_idempotent_absr, initialize_establishes_absr; propositional.
     unfold initialize.
     Split.
     - rew H.
@@ -279,13 +282,15 @@ Section Layers.
         apply to_any.
   Qed.
 
+  Hint Unfold initialize_establishes_absr : relation_rewriting.
+
   Theorem complete_exec_ok : forall T (p: a_proc T),
-      test c_initP;; inited <- initialize; ifInit inited (c_exec (compile p)) --->
+      test c_initP;; inited <- initialize rf.(impl); ifInit inited (c_exec (compile p)) --->
            (any (T:=unit);; test a_initP;; v <- a_sem.(exec) p; any (T:=unit);; pure (Some v)) +
       (any (T:=unit);; pure None).
   Proof.
     intros.
-    left_assoc rew initialize_ok.
+    left_assoc rew init_ok.
     repeat rew bind_dist_r.
     simpl.
     Split.
@@ -299,12 +304,13 @@ Section Layers.
   Qed.
 
   Theorem complete_rexec_ok : forall T (p: a_proc T) R (rec: a_proc R),
-      test c_initP;; inited <- initialize; ifInit inited (c_sem.(rexec) (compile p) (compile_rec rec)) --->
-           (any (T:=unit);; test a_initP;; v <- a_sem.(rexec) p rec; any (T:=unit);; pure (Some v)) +
-      (any (T:=unit);; pure None).
+      test c_initP;; inited <- initialize rf.(impl);
+        ifInit inited (c_sem.(rexec) (compile p) (compile_rec rec)) --->
+               (any (T:=unit);; test a_initP;; v <- a_sem.(rexec) p rec; any (T:=unit);; pure (Some v)) +
+        (any (T:=unit);; pure None).
   Proof.
     intros.
-    left_assoc rew initialize_ok.
+    left_assoc rew init_ok.
     repeat rew bind_dist_r.
     simpl.
     Split.
@@ -318,12 +324,13 @@ Section Layers.
   Qed.
 
   Theorem complete_exec_seq_ok : forall R (p: a_proc_seq R) (rec: a_proc R),
-      test c_initP;; inited <- initialize; ifInit inited (c_sem.(exec_seq) (compile_seq p) (compile_rec rec)) --->
-           (any (T:=unit);; test a_initP;; v <- a_sem.(exec_seq) p rec; any (T:=unit);; pure (Some v)) +
-      (any (T:=unit);; pure None).
+      test c_initP;; inited <- initialize rf.(impl);
+        ifInit inited (c_sem.(exec_seq) (compile_seq p) (compile_rec rec)) --->
+               (any (T:=unit);; test a_initP;; v <- a_sem.(exec_seq) p rec; any (T:=unit);; pure (Some v)) +
+        (any (T:=unit);; pure None).
   Proof.
     intros.
-    left_assoc rew initialize_ok.
+    left_assoc rew init_ok.
     repeat rew bind_dist_r.
     simpl.
     Split.
@@ -340,7 +347,7 @@ Section Layers.
   Theorem complete_exec_seq_ok_alt R (p: a_proc_seq R) (rec: a_proc R)
       (cs1 cs2: CState) mv:
     c_initP cs1 ->
-    (inited <- initialize;
+    (inited <- initialize rf.(impl);
      match inited with
      | InitFailed => pure None
      | Initialized =>
@@ -366,7 +373,7 @@ Section Layers.
   Qed.
 
   Theorem complete_exec_seq_ok_alt2 R (p: a_proc_seq R) (rec: a_proc R) v:
-    c_output (inited <- initialize;
+    c_output (inited <- initialize rf.(impl);
                 match inited with
                 | InitFailed => pure None
                 | Initialized =>
@@ -402,6 +409,31 @@ Proof.
          |}.
 Defined.
 
+Theorem initialize_simplify
+           Op1 (l1: Layer Op1) Op2
+           (impl: LayerImpl Op1 Op2) :
+  initialize l1 impl <--->
+                           exec_recover l1 impl.(init).
+Proof.
+  unfold initialize, rexec, exec_recover.
+  setoid_rewrite star_expand at 2; norm.
+  rew bind_dist_r.
+Qed.
+
+Hint Unfold initialize_establishes_absr : relation_rewriting.
+
+Lemma rexec_init_check_status:
+  forall (Op1 : Type -> Type) (l1 : Layer Op1) (Op2 : Type -> Type) (l2 : Layer Op2) (Op3 : Type -> Type)
+    (l3 : Layer Op3) (rf1 : LayerRefinement l1 l2) (rf2 : LayerRefinement l2 l3) (v : InitStatus),
+    rexec l1 (if v then compile rf1 rf2.(init) else Ret InitFailed) rf1.(init) <--->
+    (if v then rexec l1 (compile rf1 rf2.(init)) rf1.(init)
+     else _ <- l1.(crash_step); exec_recover l1 rf1.(init)).
+Proof.
+  intros Op1 l1 Op2 l2 Op3 l3 rf1 rf2 v.
+  unfold rexec.
+  destruct v; simpl; norm.
+Qed.
+
 Definition layer_compose
            Op1 (l1: Layer Op1)
            Op2 (l2: Layer Op2)
@@ -418,7 +450,7 @@ Definition layer_compose
 Proof.
   refine {| impl := layer_impl_compose rf1.(impl) rf2.(impl);
             absr := rf2.(absr);; rf1.(absr) |}.
-    simpl; intros.
+  simpl; intros.
   - (* op crash refinement *)
     red; unfold layer_impl_compose; simpl.
     split; simpl; unfold refines; norm.
@@ -440,23 +472,19 @@ Proof.
     rew H.
     rew rf1.(rexec_star_rec).
     left_assoc rew rf2.(crash_step_refinement).
-  - unfold init_establishes_absr; split.
-    + unfold layer_impl_compose; simpl.
-    +
-      rewrite <- bind_assoc.
-      rew initialize_ok.
-      Split.
-      * rew rf1.(compile_exec_ok).
-        setoid_rewrite <- bind_assoc at 2.
-        rew rf2.(init_ok).
-        repeat (setoid_rewrite bind_dist_r ||
-                setoid_rewrite bind_dist_l); norm.
-        left_assoc rew any_idem.
-        Split.
-        -- Left.
-        -- Right.
-           rewrite <- bind_assoc.
-           rel_congruence.
-           apply to_any.
-      * Right.
-Qed.
+  - unfold initialize_establishes_absr.
+    rew initialize_simplify.
+    simpl.
+    rew @exec_recover_bind.
+    rew<- initialize_simplify.
+    rewrite <- bind_assoc.
+    rew rf1.(init_ok).
+    Split.
+    + rew rexec_init_check_status.
+    (* need some bind_star induction *)
+      admit.
+    + Right.
+      (* similar bind_star induction (but much simpler because it just reduces
+      to pure InitFailed) *)
+      admit.
+Admitted.
